C-verifier/src/Midend-IVL/Isabelle-UTP-Extended/case_studies/TotalCorrectness/Abrupt/cJSON/cJSON.thy
@@ -62,6 +62,7 @@ record '\<alpha> internal_hooks =
 type_synonym cJSON_bool = int
 
 type_synonym '\<alpha> str_lens = \<open>string option \<Longrightarrow> '\<alpha>\<close>
+type_synonym '\<alpha> str_expr = \<open>(string option, '\<alpha>) uexpr\<close>
 
 subsection \<open>From source file \texttt{cJSON.c}\<close>
 
@@ -81,7 +82,10 @@ record '\<alpha> parse_buffer =
   hooks :: \<open>'\<alpha> internal_hooks\<close>
 
 type_synonym '\<alpha> parse_buffer_lens = \<open>'\<alpha> parse_buffer option \<Longrightarrow> '\<alpha>\<close>
+type_synonym '\<alpha> parse_buffer_expr = \<open>('\<alpha> parse_buffer option, '\<alpha>) uexpr\<close>
 
+(* TODO: Need a mutable setup because we're verifying C and C expects buffer' to be a set buffer
+that can be modified, not a list to be replaced with new versions. *)
 record '\<alpha> printbuffer =
   buffer' :: \<open>'\<alpha> str_lens\<close>
   length' :: size_t
@@ -101,34 +105,40 @@ definition \<open>cJSON_Version = shows\<^sub>u(CJSON_VERSION_MAJOR) ^\<^sub>u \
                             shows\<^sub>u(CJSON_VERSION_MINOR) ^\<^sub>u \<guillemotleft>''.''\<guillemotright> ^\<^sub>u
                             shows\<^sub>u(CJSON_VERSION_PATCH)\<close>
 
+(* TODO: global/local variable differentiation? *)
 locale cJSON =
   fixes int_ret :: \<open>int \<Longrightarrow> '\<alpha>\<close>
-    and tempstr\<^sub>1 tempstr\<^sub>2 :: \<open>string \<Longrightarrow> '\<alpha>\<close> \<comment> \<open>Assuming already shown non-@{const None}\<close>
-  assumes \<open>vwb_lens int_ret\<close>
+    and nat_ret :: \<open>nat \<Longrightarrow> '\<alpha>\<close>
+    and tempstr\<^sub>1 :: \<open>string \<Longrightarrow> '\<alpha>\<close> \<comment> \<open>Assuming already shown non-@{const None}\<close>
+    and tempstr\<^sub>2
+  assumes INDEP: \<open>vwb_lens int_ret\<close> \<open>vwb_lens nat_ret\<close>
           \<open>lens_indep_all [tempstr\<^sub>1, tempstr\<^sub>2]\<close>
+          \<open>int_ret \<bowtie> tempstr\<^sub>1\<close> \<open>int_ret \<bowtie> tempstr\<^sub>2\<close>
+          \<open>int_ret \<bowtie> nat_ret\<close>
+          \<open>nat_ret \<bowtie> tempstr\<^sub>1\<close> \<open>nat_ret \<bowtie> tempstr\<^sub>2\<close>
 begin
 
 (* TODO: Block or frame? *)
-definition case_insensitive_strcmp :: \<open>'\<alpha> str_lens \<Rightarrow> '\<alpha> str_lens \<Rightarrow> '\<alpha> hrel_cpa\<close> where
+definition case_insensitive_strcmp :: \<open>'\<alpha> str_expr \<Rightarrow> '\<alpha> str_expr \<Rightarrow> '\<alpha> hrel_cpa\<close> where
   \<open>case_insensitive_strcmp string\<^sub>1 string\<^sub>2 \<equiv>
 try
-  bif &string\<^sub>1 =\<^sub>u \<guillemotleft>None\<guillemotright> \<or> &string\<^sub>2 =\<^sub>u \<guillemotleft>None\<guillemotright> then
+  bif string\<^sub>1 =\<^sub>u \<guillemotleft>None\<guillemotright> \<or> string\<^sub>2 =\<^sub>u \<guillemotleft>None\<guillemotright> then
     int_ret \<Midarrow> 1;;
     THROW\<^sub>A\<^sub>B\<^sub>R
   else II eif;;
-  bif &string\<^sub>1 =\<^sub>u &string\<^sub>2 then
+  bif string\<^sub>1 =\<^sub>u string\<^sub>2 then
     int_ret \<Midarrow> 0;;
     THROW\<^sub>A\<^sub>B\<^sub>R
   else II eif;;
-  tempstr\<^sub>1 \<Midarrow> lowercase\<^sub>u (the\<^sub>u (&string\<^sub>1));;
-  tempstr\<^sub>2 \<Midarrow> lowercase\<^sub>u (the\<^sub>u (&string\<^sub>2));;
+  tempstr\<^sub>1 \<Midarrow> lowercase\<^sub>u (the\<^sub>u string\<^sub>1);;
+  tempstr\<^sub>2 \<Midarrow> lowercase\<^sub>u (the\<^sub>u string\<^sub>2);;
   while head\<^sub>u(&tempstr\<^sub>1) =\<^sub>u head\<^sub>u(&tempstr\<^sub>2)
-  invr #\<^sub>u(&tempstr\<^sub>1) \<le>\<^sub>u #\<^sub>u(the\<^sub>u (&string\<^sub>1)) \<and> #\<^sub>u(&tempstr\<^sub>2) \<le>\<^sub>u #\<^sub>u(the\<^sub>u (&string\<^sub>2)) do (* TODO: probably needs more/something else, might require extra ghost variable *)
+  invr #\<^sub>u(&tempstr\<^sub>1) \<le>\<^sub>u #\<^sub>u(the\<^sub>u string\<^sub>1) \<and> #\<^sub>u(&tempstr\<^sub>2) \<le>\<^sub>u #\<^sub>u(the\<^sub>u string\<^sub>2) do (* TODO: probably needs more/something else, might require extra ghost variable *)
     bif #\<^sub>u(&tempstr\<^sub>1) =\<^sub>u 0 then (* Strings here aren't null-terminated *)
       int_ret \<Midarrow> 0;;
       THROW\<^sub>A\<^sub>B\<^sub>R  
     else II eif;;
-    (#\<^sub>u(&tempstr\<^sub>1) \<le>\<^sub>u #\<^sub>u(the\<^sub>u (&string\<^sub>2)) \<and> #\<^sub>u(&tempstr\<^sub>2) \<le>\<^sub>u #\<^sub>u(the\<^sub>u (&string\<^sub>2)))\<^sub>\<bottom>\<^sub>C;;
+    (#\<^sub>u(&tempstr\<^sub>1) \<le>\<^sub>u #\<^sub>u(the\<^sub>u string\<^sub>2) \<and> #\<^sub>u(&tempstr\<^sub>2) \<le>\<^sub>u #\<^sub>u(the\<^sub>u string\<^sub>2))\<^sub>\<bottom>\<^sub>C;;
     tempstr\<^sub>1 \<Midarrow> tail\<^sub>u(&tempstr\<^sub>1);;
     tempstr\<^sub>2 \<Midarrow> tail\<^sub>u(&tempstr\<^sub>2)
   od;;
@@ -143,24 +153,69 @@ end
 (* TODO: get_decimal_point (needs locale access somehow? or just nondeterminism) *)
 
 text \<open>Check if the given size is left to read in a given parse buffer (starting with 1)\<close>
-abbreviation can_read ::
-  \<open>('\<alpha> parse_buffer option, '\<alpha>) uexpr \<Rightarrow> (size_t, '\<alpha>) uexpr \<Rightarrow> '\<alpha> upred\<close> where
+abbreviation can_read :: \<open>'\<alpha> parse_buffer_expr \<Rightarrow> (size_t, '\<alpha>) uexpr \<Rightarrow> '\<alpha> upred\<close> where
   \<open>can_read buffer size' \<equiv> buffer \<noteq>\<^sub>u \<guillemotleft>None\<guillemotright> \<and>
                            (the\<^sub>u buffer)\<lparr>offset\<rparr>\<^sub>r + size' \<le>\<^sub>u (the\<^sub>u buffer)\<lparr>length\<rparr>\<^sub>r\<close>
-abbreviation \<open>cannot_read buffer size'\<equiv> \<not> can_read buffer size'\<close>
+abbreviation \<open>cannot_read buffer size' \<equiv> \<not> can_read buffer size'\<close>
 
 text \<open>Check if the buffer can be accessed at the given index (starting with 0)\<close>
-abbreviation can_access_at_index ::
-  \<open>('\<alpha> parse_buffer option, '\<alpha>) uexpr \<Rightarrow> (size_t, '\<alpha>) uexpr \<Rightarrow> '\<alpha> upred\<close> where
+abbreviation can_access_at_index :: \<open>'\<alpha> parse_buffer_expr \<Rightarrow> (size_t, '\<alpha>) uexpr \<Rightarrow> '\<alpha> upred\<close> where
   \<open>can_access_at_index buffer index \<equiv> buffer \<noteq>\<^sub>u \<guillemotleft>None\<guillemotright> \<and>
                                       (the\<^sub>u buffer)\<lparr>offset\<rparr>\<^sub>r + index \<le>\<^sub>u (the\<^sub>u buffer)\<lparr>length\<rparr>\<^sub>r\<close>
-abbreviation \<open>cannot_access_at_index buffer index\<equiv> \<not> can_access_at_index buffer index\<close>
+abbreviation \<open>cannot_access_at_index buffer index \<equiv> \<not> can_access_at_index buffer index\<close>
 
 (* TODO: figure out buffer_at_offset when using memory model; arrays are usually mutable but
 Isabelle lists/etc. are not and we can't just return a reference to the remnant of the list/string.
 *)
 (* TODO: parse_number *)
+(* TODO: ensure *)
+(* TODO: update_offset; not be necessary when not working with actual pointers *)
+(* TODO: print_number; has some stuff involving C-specific number handling *)
 
+end
+
+text \<open>Creating locale extensions for individual functions as necessary.\<close>
+locale parse_hex4 = cJSON +
+  constrains int_ret :: \<open>int \<Longrightarrow> '\<alpha>\<close> \<comment> \<open>@{typ '\<alpha>} not propagated from base locale.\<close>
+         and tempstr\<^sub>1 :: \<open>string \<Longrightarrow> '\<alpha>\<close>
+         and tempstr\<^sub>2 :: \<open>string \<Longrightarrow> '\<alpha>\<close>
+  fixes h i chari and tinput :: \<open>string \<Longrightarrow> '\<alpha>\<close>
+  assumes INDEP: \<open>lens_indep_all [nat_ret, h, i, chari]\<close>
+          \<open>int_ret \<bowtie> h\<close> \<open>int_ret \<bowtie> i\<close>
+          \<open>int_ret \<bowtie> tinput\<close>
+begin
+
+text \<open>parse 4 digit hexadecimal number\<close>
+definition parse_hex4 :: \<open>'\<alpha> str_expr \<Rightarrow> '\<alpha> hrel_cpa\<close> where
+  \<open>parse_hex4 input \<equiv>
+h \<Midarrow> 0;;
+i \<Midarrow> 0;;
+tinput \<Midarrow> the\<^sub>u input;; (* Assumes not NULL/None *)
+try
+  while &i <\<^sub>u 4 invr true do (* TODO: invariant; assumes input has at least 4 chars *)
+    chari \<Midarrow> nat_of_char\<^sub>u (&tinput(&i)\<^sub>a);;
+    bif &chari \<ge>\<^sub>u \<guillemotleft>nat_of_char CHR ''0''\<guillemotright> then
+      h \<Midarrow> (&h + &chari - \<guillemotleft>nat_of_char CHR ''0''\<guillemotright>)
+    else
+      bif &chari \<ge>\<^sub>u \<guillemotleft>nat_of_char CHR ''A''\<guillemotright> \<and> &chari \<le>\<^sub>u \<guillemotleft>nat_of_char CHR ''F''\<guillemotright> then
+        h \<Midarrow> (&h + 10 + &chari - \<guillemotleft>nat_of_char CHR ''A''\<guillemotright>)
+      else
+        bif &chari \<ge>\<^sub>u \<guillemotleft>nat_of_char CHR ''a''\<guillemotright> \<and> &chari \<le>\<^sub>u \<guillemotleft>nat_of_char CHR ''f''\<guillemotright> then
+          h \<Midarrow> (&h + 10 + &chari - \<guillemotleft>nat_of_char CHR ''a''\<guillemotright>)
+        else
+          nat_ret \<Midarrow> 0;;
+          THROW\<^sub>A\<^sub>B\<^sub>R
+        eif
+      eif
+    eif;; (* TODO: assertion? *)
+    bif &i <\<^sub>u 3 then
+      h \<Midarrow> &h \<lless>\<^bsub>u/SIZEOF_INT\<^esub> 4 (* shift left to make place for the next nibble *)
+    else II eif (* TODO: assertion? *)
+  od
+catch
+  II
+end
+\<close>
 
 end
 
